WIP example 2.5 TypingStep seems to be usable as is using `rw!` instead of rw.

PiLL/PiLL/Alt.lean
@@ -1,96 +1,97 @@
 import Mathlib.Data.Finset.Basic
 import Mathlib.Data.Finset.Card
 import Mathlib.Data.Finset.Fold
+import Mathlib.Tactic
 
-abbrev PName := Nat
+-- abbrev PName := Nat
 
-inductive Proc : Type where
-  | tensor  (x y : PName) (P : Proc)
-  | parr    (x y : PName) (P : Proc)
-  | one     (x : PName) (P : Proc)
-  | bot     (x : PName) (P : Proc)
-  | cut     (x y : PName) (P : Proc)
-  | par     (P Q : Proc)
-  | nil
-deriving DecidableEq
+-- inductive Proc : Type where
+--   | tensor  (x y : PName) (P : Proc)
+--   | parr    (x y : PName) (P : Proc)
+--   | one     (x : PName) (P : Proc)
+--   | bot     (x : PName) (P : Proc)
+--   | cut     (x y : PName) (P : Proc)
+--   | par     (P Q : Proc)
+--   | nil
+-- deriving DecidableEq
 
-abbrev Atom := Nat
+-- abbrev Atom := Nat
 
-inductive Types : Type where
-  | atom      (a : Atom)
-  | atomDual  (a : Atom)
-  | tensor    (A B : Types)
-  | parr      (A B : Types)
-  | one
-  | bot
-deriving DecidableEq
+-- inductive Types : Type where
+--   | atom      (a : Atom)
+--   | atomDual  (a : Atom)
+--   | tensor    (A B : Types)
+--   | parr      (A B : Types)
+--   | one
+--   | bot
+-- deriving DecidableEq
 
-abbrev Env := Finset (PName × Types)
+-- abbrev Env := Finset (PName × Types)
 
-abbrev HyperEnv := Finset (Env)
+-- abbrev HyperEnv := Finset (Env)
 
-inductive Act : Type
-  | one     (x : PName)
-  | bot     (x : PName)
-  | tensor  (x y : PName)
-  | parr    (x y : PName)
-deriving Repr, DecidableEq
+-- inductive Act : Type
+--   | one     (x : PName)
+--   | bot     (x : PName)
+--   | tensor  (x y : PName)
+--   | parr    (x y : PName)
+-- deriving Repr, DecidableEq
 
-inductive Lbl : Type
-  | tau
-  | act   (a : Act)
-  | par   (l l' : Act)
-deriving Repr, DecidableEq
+-- inductive Lbl : Type
+--   | tau
+--   | act   (a : Act)
+--   | par   (l l' : Act)
+-- deriving Repr, DecidableEq
 
-theorem swap_last (A B C : Env) : A ∪ B ∪ C = A ∪ C ∪ B := by
-  rw [Finset.union_assoc, Finset.union_comm B C, Finset.union_assoc]
+-- theorem swap_last (A B C : Env) : A ∪ B ∪ C = A ∪ C ∪ B := by
+--   rw [Finset.union_assoc, Finset.union_comm B C, Finset.union_assoc]
 
-theorem move_last_two_forward (A B C D : Env) : ((A ∪ B) ∪ C) ∪ D = ((A ∪ D) ∪ B) ∪ C := by
-  rw [Finset.union_assoc A B C, swap_last, ← Finset.union_assoc]
+-- theorem move_last_two_forward (A B C D : Env) : ((A ∪ B) ∪ C) ∪ D = ((A ∪ D) ∪ B) ∪ C := by
+--   rw [Finset.union_assoc A B C, swap_last, ← Finset.union_assoc]
 
-inductive Typing : HyperEnv → Proc → Prop where
-  | bot {Γ : Env} {P : Proc} {x : PName} : -- {A : Types} :
-      Typing {Γ} P →
-      Typing {Γ ∪ {(x, Types.bot)}} (Proc.bot x P)
+-- inductive Typing : HyperEnv → Proc → Prop where
+--   | bot {Γ : Env} {P : Proc} {x : PName} : -- {A : Types} :
+--       Typing {Γ} P →
+--       Typing {Γ ∪ {(x, Types.bot)}} (Proc.bot x P)
 
-  | parr {Γ : Env} {P : Proc} {x y : PName} {A B : Types} :
-      Typing {Γ ∪ {(y, A)} ∪ {(x, B)}} P →
-      Typing {Γ ∪ {(x, A.parr B)}} (Proc.parr x y P)
+--   | parr {Γ : Env} {P : Proc} {x y : PName} {A B : Types} :
+--       Typing {Γ ∪ {(y, A)} ∪ {(x, B)}} P →
+--       Typing {Γ ∪ {(x, A.parr B)}} (Proc.parr x y P)
 
-inductive TypingStep : HyperEnv → Proc → Lbl →
-  HyperEnv → Proc → Prop where
-   | bot
-      {Γ : Env} {P : Proc} {x : Nat}
-      (𝒟 : Typing {Γ ∪ {(x, Types.bot)}} (Proc.bot x P))
-      (𝒟' : Typing {Γ} P) :
-      TypingStep
-        {Γ ∪ {(x, Types.bot)}} (Proc.bot x P)
-        (Lbl.act (Act.bot x))
-        {Γ} P
+-- inductive TypingStep : HyperEnv → Proc → Lbl →
+--   HyperEnv → Proc → Prop where
+--    | bot
+--       {Γ : Env} {P : Proc} {x : Nat}
+--       (𝒟 : Typing {Γ ∪ {(x, Types.bot)}} (Proc.bot x P))
+--       (𝒟' : Typing {Γ} P) :
+--       TypingStep
+--         {Γ ∪ {(x, Types.bot)}} (Proc.bot x P)
+--         (Lbl.act (Act.bot x))
+--         {Γ} P
 
-  | parr
-      {Γ : Env} {P : Proc} {x y : Nat} {A B : Types}
-      (𝒟 : Typing {Γ ∪ {(x, A.parr B)}} (Proc.parr x y P))
-      (𝒟' : Typing {Γ ∪ {(y, A)} ∪ {(x, B)}} P) :
-      TypingStep
-        {Γ ∪ {(x, A.parr B)}} (Proc.parr x y P)
-        (Lbl.act (Act.parr x y))
-        {Γ ∪ {(y, A)} ∪ {(x, B)}} P
+--   | parr
+--       {Γ : Env} {P : Proc} {x y : Nat} {A B : Types}
+--       (𝒟 : Typing {Γ ∪ {(x, A.parr B)}} (Proc.parr x y P))
+--       (𝒟' : Typing {Γ ∪ {(y, A)} ∪ {(x, B)}} P) :
+--       TypingStep
+--         {Γ ∪ {(x, A.parr B)}} (Proc.parr x y P)
+--         (Lbl.act (Act.parr x y))
+--         {Γ ∪ {(y, A)} ∪ {(x, B)}} P
 
-example {Γ : Env} {P : Proc} {x y z : PName} {A B : Types}
-  (𝒟 : Typing {Γ ∪ {(x, A.parr B)} ∪ {(z, Types.bot)}} (Proc.parr x y (Proc.bot z P)))
-  (𝒟' : Typing {Γ ∪ {(y, A)} ∪ {(x, B)} ∪ {(z, Types.bot)}} (Proc.bot z P)) :
-  TypingStep
-    {Γ ∪ {(x, A.parr B)} ∪ {(z, Types.bot)}} (Proc.parr x y (Proc.bot z P))
-    (Lbl.act (Act.parr x y))
-    {Γ ∪ {(y, A)} ∪ {(x, B)} ∪ {(z, Types.bot)}} (Proc.bot z P) := by
+-- example {Γ : Env} {P : Proc} {x y z : PName} {A B : Types}
+--   (𝒟 : Typing {Γ ∪ {(x, A.parr B)} ∪ {(z, Types.bot)}} (Proc.parr x y (Proc.bot z P)))
+--   (𝒟' : Typing {Γ ∪ {(y, A)} ∪ {(x, B)} ∪ {(z, Types.bot)}} (Proc.bot z P)) :
+--   TypingStep
+--     {Γ ∪ {(x, A.parr B)} ∪ {(z, Types.bot)}} (Proc.parr x y (Proc.bot z P))
+--     (Lbl.act (Act.parr x y))
+--     {Γ ∪ {(y, A)} ∪ {(x, B)} ∪ {(z, Types.bot)}} (Proc.bot z P) := by
 
-  rw [swap_last, move_last_two_forward]
-  apply TypingStep.parr
-  · rw [← swap_last]
-    exact 𝒟
-  · rw [← move_last_two_forward]
-    exact 𝒟'
+--   rw [swap_last, move_last_two_forward]
+--   apply TypingStep.parr
+--   · rw [← swap_last]
+--     exact 𝒟
+--   · rw [← move_last_two_forward]
+--     exact 𝒟'
 
 
 
@@ -177,57 +178,58 @@ example {Γ : Env} {P : Proc} {x y z : PName} {A B : Types}
 
 
 /- Zulip example -/
--- abbrev Env := Finset (Nat × Nat)
--- abbrev HyperEnv := Finset (Env)
+abbrev Env := Finset (Nat × Nat)
+abbrev HyperEnv := Finset (Env)
 
--- inductive Typing : HyperEnv → Prop where
---   | parr {Γ : Env} {x y A B : Nat} :
---       Typing {Γ ∪ {(y, A)} ∪ {(x, B)}} →
---       Typing {Γ ∪ {(x, A + B)}}
+inductive Typing : HyperEnv → Prop where
+  | parr {Γ : Env} {x y A B : Nat} :
+      Typing {Γ ∪ {(y, A)} ∪ {(x, B)}} →
+      Typing {Γ ∪ {(x, A + B)}}
 
--- inductive TS1 : HyperEnv → List (Nat × Nat) →
---   HyperEnv → Prop where
---   | parr
---       {Γ : Env} {x y A B : Nat}
---       (𝒟 : Typing {Γ ∪ {(x, A + B)}})
---       (𝒟' : Typing {Γ ∪ {(y, A)} ∪ {(x, B)}}) :
---       TS1
---         {Γ ∪ {(x, A + B)}}
---         [(x, y)]
---         {Γ ∪ {(y, A)} ∪ {(x, B)}}
+inductive TS1 : HyperEnv → List (Nat × Nat) →
+  HyperEnv → Prop where
+  | parr
+      {Γ : Env} {x y A B : Nat}
+      (𝒟 : Typing {Γ ∪ {(x, A + B)}})
+      (𝒟' : Typing {Γ ∪ {(y, A)} ∪ {(x, B)}}) :
+      TS1
+        {Γ ∪ {(x, A + B)}}
+        [(x, y)]
+        {Γ ∪ {(y, A)} ∪ {(x, B)}}
 
--- inductive TS2 : ∀ {𝒢 𝒢' : HyperEnv},
---   Typing 𝒢 → List (Nat × Nat) → Typing 𝒢' → Prop where
---   | parr
---       {Γ : Env} {x y A B : Nat}
---       (𝒟 : Typing {Γ ∪ {(y, A)} ∪ {(x, B)}}) :
---       TS2
---         (Typing.parr 𝒟)
---         [(x, y)]
---         𝒟
+inductive TS2 : ∀ {𝒢 𝒢' : HyperEnv},
+  Typing 𝒢 → List (Nat × Nat) → Typing 𝒢' → Prop where
+  | parr
+      {Γ : Env} {x y A B : Nat}
+      (𝒟 : Typing {Γ ∪ {(y, A)} ∪ {(x, B)}}) :
+      TS2
+        (Typing.parr 𝒟)
+        [(x, y)]
+        𝒟
 
--- theorem swap_last_two (A B C : Env) : A ∪ B ∪ C = A ∪ C ∪ B := by aesop
--- theorem move_last_two_left (A B C D : Env) : A ∪ B ∪ C ∪ D = A ∪ D ∪ B ∪ C := by aesop
+theorem swap_last_two (A B C : Env) : A ∪ B ∪ C = A ∪ C ∪ B := by aesop
+theorem move_last_two_left (A B C D : Env) : A ∪ B ∪ C ∪ D = A ∪ D ∪ B ∪ C := by aesop
 
--- theorem example1 {Γ : Env} {x y z A B : Nat}
---   (𝒟 : Typing {Γ ∪ {(x, A + B)} ∪ {(z, 0)}})
---   (𝒟' : Typing {Γ ∪ {(y, A)} ∪ {(x, B)} ∪ {(z, 0)}}) :
---   TS1
---     {Γ ∪ {(x, A + B)} ∪ {(z, 0)}}
---     [(x, y)]
---     {Γ ∪ {(y, A)} ∪ {(x, B)} ∪ {(z, 0)}} := by
---   rw [move_last_two_left]
---   rw [swap_last_two]
---   apply TS1.parr
---   · rw [← swap_last_two] ; exact 𝒟
---   · rw [← move_last_two_left] ; exact 𝒟'
+theorem example1 {Γ : Env} {x y z A B : Nat}
+  (𝒟 : Typing {Γ ∪ {(x, A + B)} ∪ {(z, 0)}})
+  (𝒟' : Typing {Γ ∪ {(y, A)} ∪ {(x, B)} ∪ {(z, 0)}}) :
+  TS1
+    {Γ ∪ {(x, A + B)} ∪ {(z, 0)}}
+    [(x, y)]
+    {Γ ∪ {(y, A)} ∪ {(x, B)} ∪ {(z, 0)}} := by
+  rw [move_last_two_left]
+  rw [swap_last_two]
+  apply TS1.parr
+  · rw [← swap_last_two] ; exact 𝒟
+  · rw [← move_last_two_left] ; exact 𝒟'
 
--- theorem example2 {Γ : Env} {x y z A B : Nat}
---   (𝒟 : Typing {Γ ∪ {(y, A)} ∪ {(x, B)} ∪ {(z, 0)}}) :
---   TS2
---     (Typing.parr 𝒟)
---     [(x, y)]
---     𝒟 := by
---   rw [swap_last_two] at 𝒟 -- Creates a copy instead of rewriting the goal
---   rw [move_last_two_left] -- Tactic `rewrite` failed: motive is not type correct
---   sorry
+theorem example2 {Γ : Env} {x y z A B : Nat}
+  (𝒟 : Typing {Γ ∪ {(x, A + B)} ∪ {(z, 0)}})
+  (𝒟' : Typing {Γ ∪ {(y, A)} ∪ {(x, B)} ∪ {(z, 0)}}) :
+  TS2
+    𝒟
+    [(x, y)]
+    𝒟' := by
+  rw! [swap_last_two]
+  rw! [move_last_two_left]
+  apply TS2.parr
